ModularEngine/src/LogicEngine.FStar/prims.fst
@@ -180,6 +180,8 @@ extern Runtime val strSubstring: string -> int -> int -> string
 extern Runtime val strSubstringNoLength: string -> int -> string
 extern Runtime val strIndexOf: string -> string -> int
 extern Runtime val strLastIndexOf: string -> string -> int
+extern Runtime val strLength: string -> int
+extern Runtime val strTrim: string -> string
 
 extern Runtime val boxToObject: 'a -> object
 extern Runtime val addBindings: object -> string -> bool
